\documentclass{beamer}

\usepackage{pr√©ambule}

\begin{document}

\begin{frame}
	Simplifier au maximum les expressions ci-dessous :
	\begin{enumerate}
		\item $\vec{AC} + \vec{CD} + \vec{DE} = \correction{\vec{AE}}$
		\item $\vec{FE} - \vec{CD} + \vec{ED} = \correction{\vec{FC}}$
		\item $\vec{EA} - (\vec{EC} + \vec{ED}) + \vec{AD} = $
		\item $\vec{AE} + \vec{TA} + \vec{FT} + \vec{EF} = \correction{\vec{0}}$
	\end{enumerate}
\end{frame}

\begin{frame}
	Simplifier au maximum les expressions ci-dessous :
	\begin{enumerate}
		\item $2\vec{AC} + 2\vec{CD} + 2\vec{DE} = \correction{2\vec{AE}}$
		\item $\vec{AC} + 2\vec{CD} + \vec{DA} = \correction{2\vec{AE}}$
		\item $7(\vec{u} + \vec{v}) - 3\vec{v} = \correction{7\vec{u} + 4\vec{v}}$
		\item $\dfrac{1}{2}\vec{CE} - 2\vec{BE} - \dfrac{1}{2}\vec{CB} = \correction{\dfrac{3}{2}\vec{EB}}$
	\end{enumerate}
\end{frame}

\end{document}